

Antoni Iwanowski  
Nr indeksu: 479235

## Zadanie 1

Przekształcamy (i) równoważnie.

$$\begin{aligned}
|z - w| &< |1 - z\bar{w}| \\
|z - w|^2 &< |1 - z\bar{w}|^2 \\
(z - w)(\overline{z - w}) &< (1 - z\bar{w})(\overline{1 - z\bar{w}}) \\
(z - w)(\bar{z} - \bar{w}) &< (1 - z\bar{w})(1 - \overline{z\bar{w}}) \\
(z - w)(\bar{z} - \bar{w}) &< (1 - z\bar{w})(1 - \bar{z}w) \\
z\bar{z} - z\bar{w} - w\bar{z} + w\bar{w} &< 1 - \bar{z}w - z\bar{w} + z\bar{z}w\bar{w} \\
z\bar{z} + w\bar{w} &< 1 + z\bar{z}w\bar{w} \\
0 &< z\bar{z}w\bar{w} - z\bar{z} + 1 - w\bar{w} \\
0 &< z\bar{z}(w\bar{w} - 1) - (w\bar{w} - 1) \\
0 &< (z\bar{z} - 1)(w\bar{w} - 1) \\
0 &< (|z|^2 - 1)(|w|^2 - 1) \\
((|z|^2 - 1 > 0) \wedge (|w|^2 - 1 > 0)) &\vee ((|z|^2 - 1 < 0) \wedge (|w|^2 - 1 < 0)) \\
((|z|^2 > 1) \wedge (|w|^2 > 1)) &\vee ((|z|^2 < 1) \wedge (|w|^2 < 1)) \\
((|z| > 1) \wedge (|w| > 1)) &\vee ((|z| < 1) \wedge (|w| < 1))
\end{aligned}$$

Przekształcając (i) równoważnie otrzymaliśmy (ii). Zatem:

$$(i) \iff (ii)$$